skeletons/skeletons.v
@@ -11,9 +11,9 @@ Require Export declarational.
 Inductive sk_vtype : Type :=
 | SkTyUnit : sk_vtype
 | SkTyInt : sk_vtype
-| SkTyØ : sk_vtype
-| SkTyΣ : sk_vtype -> sk_vtype -> sk_vtype
-| SkTyΠ : sk_vtype -> sk_vtype -> sk_vtype
+| SkTyEmpty : sk_vtype
+| SkTySum : sk_vtype -> sk_vtype -> sk_vtype
+| SkTyProd : sk_vtype -> sk_vtype -> sk_vtype
 | SkTyList : sk_vtype -> sk_vtype
 | SkTyFun : sk_vtype -> sk_ctype -> sk_vtype
 | SkTyHandler : sk_ctype -> sk_ctype -> sk_vtype
@@ -26,24 +26,24 @@ Inductive sk_val : Type :=
 | SkVar : nat -> sk_val
 | SkUnit : sk_val
 | SkInt : Z.t -> sk_val
-| SkInl : sk_val -> sk_val
-| SkInr : sk_val -> sk_val
+| SkLeft : sk_val -> sk_val
+| SkRight : sk_val -> sk_val
 | SkPair : sk_val -> sk_val -> sk_val
-| SkListNil : sk_val
-| SkListCons : sk_val -> sk_val -> sk_val
+| SkNil : sk_val
+| SkCons : sk_val -> sk_val -> sk_val
 | SkFun : sk_comp -> sk_val
 | SkHandler : sk_comp -> sk_hcases -> sk_val
 
 with sk_comp : Type :=
 | SkRet : sk_val -> sk_comp
 | SkAbsurd : sk_val -> sk_comp
-| SkΠMatch : sk_val -> sk_comp -> sk_comp
-| SkΣMatch : sk_val -> sk_comp -> sk_comp -> sk_comp
+| SkProdMatch : sk_val -> sk_comp -> sk_comp
+| SkSumMatch : sk_val -> sk_comp -> sk_comp -> sk_comp
 | SkListMatch : sk_val -> sk_comp -> sk_comp -> sk_comp
 | SkApp : sk_val -> sk_val -> sk_comp
 | SkOp : op_id -> sk_vtype -> sk_vtype -> sk_val -> sk_comp -> sk_comp
 | SkLetRec : sk_comp -> sk_comp -> sk_comp
-| SkDoBind : sk_comp -> sk_comp -> sk_comp
+| SkDo : sk_comp -> sk_comp -> sk_comp
 | SkHandle : sk_val -> sk_comp -> sk_comp
 
 with sk_hcases : Type :=
@@ -76,19 +76,19 @@ Inductive has_sk_vtype : sk_ctx -> sk_val -> sk_vtype -> Prop :=
 | SkTypePair Γ v1 v2 A B :
     has_sk_vtype Γ v1 A ->
     has_sk_vtype Γ v2 B ->
-    has_sk_vtype Γ (SkPair v1 v2) (SkTyΠ A B)
-| SkTypeInl Γ v A B :
+    has_sk_vtype Γ (SkPair v1 v2) (SkTyProd A B)
+| SkTypeLeft Γ v A B :
     has_sk_vtype Γ v A ->
-    has_sk_vtype Γ (SkInl v) (SkTyΣ A B)
-| SkTypeInr Γ v A B :
+    has_sk_vtype Γ (SkLeft v) (SkTySum A B)
+| SkTypeRight Γ v A B :
     has_sk_vtype Γ v B ->
-    has_sk_vtype Γ (SkInr v) (SkTyΣ A B)
-| SkTypeListNil Γ A :
-    has_sk_vtype Γ SkListNil (SkTyList A)
-| SkTypeListCons Γ v vs A :
+    has_sk_vtype Γ (SkRight v) (SkTySum A B)
+| SkTypeNil Γ A :
+    has_sk_vtype Γ SkNil (SkTyList A)
+| SkTypeCons Γ v vs A :
     has_sk_vtype Γ v A ->
     has_sk_vtype Γ vs (SkTyList A) ->
-    has_sk_vtype Γ (SkListCons v vs) (SkTyList A)
+    has_sk_vtype Γ (SkCons v vs) (SkTyList A)
 | SkTypeFun Γ c A C :
     has_sk_ctype (SkCtxU Γ A) c C ->
     has_sk_vtype Γ (SkFun c) (SkTyFun A C)
@@ -102,26 +102,26 @@ with has_sk_ctype : sk_ctx -> sk_comp -> sk_ctype -> Prop :=
     has_sk_vtype Γ v A ->
     has_sk_ctype Γ (SkRet v) (SkCTy A)
 | SkTypeAbsurd Γ v C :
-    has_sk_vtype Γ v SkTyØ -> 
+    has_sk_vtype Γ v SkTyEmpty -> 
     has_sk_ctype Γ (SkAbsurd v) C
-| SkTypeΠMatch Γ v A B c C :
-    has_sk_vtype Γ v (SkTyΠ A B) ->
+| SkTypeProdMatch Γ v A B c C :
+    has_sk_vtype Γ v (SkTyProd A B) ->
     has_sk_ctype (SkCtxU (SkCtxU Γ A) B) c C ->
-    has_sk_ctype Γ (SkΠMatch v c) C
-| SkTypeΣMatch Γ v A B c1 c2 C :
-    has_sk_vtype Γ v (SkTyΣ A B) ->
+    has_sk_ctype Γ (SkProdMatch v c) C
+| SkTypeSumMatch Γ v A B c1 c2 C :
+    has_sk_vtype Γ v (SkTySum A B) ->
     has_sk_ctype (SkCtxU Γ A) c1 C ->
     has_sk_ctype (SkCtxU Γ B) c2 C ->
-    has_sk_ctype Γ (SkΣMatch v c1 c2) C
+    has_sk_ctype Γ (SkSumMatch v c1 c2) C
 | SkTypeListMatch Γ v A c1 c2 C :
     has_sk_vtype Γ v (SkTyList A) ->
     has_sk_ctype Γ c1 C ->
     has_sk_ctype (SkCtxU (SkCtxU Γ A) (SkTyList A)) c2 C ->
     has_sk_ctype Γ (SkListMatch v c1 c2) C
-| SkTypeDoBind Γ c1 c2 A B :
+| SkTypeDo Γ c1 c2 A B :
     has_sk_ctype Γ c1 (SkCTy A) ->
     has_sk_ctype (SkCtxU Γ A) c2 (SkCTy B) ->
-    has_sk_ctype Γ (SkDoBind c1 c2) (SkCTy B)
+    has_sk_ctype Γ (SkDo c1 c2) (SkCTy B)
 | SkTypeApp Γ v1 v2 A C :
     has_sk_vtype Γ v1 (SkTyFun A C) ->
     has_sk_vtype Γ v2 A ->
@@ -154,9 +154,9 @@ Fixpoint skeletize_vtype A :=
   match A with
   | TyUnit => SkTyUnit
   | TyInt => SkTyInt
-  | TyØ => SkTyØ
-  | TyΣ A B => SkTyΣ (skeletize_vtype A) (skeletize_vtype B)
-  | TyΠ A B => SkTyΠ (skeletize_vtype A) (skeletize_vtype B)
+  | TyEmpty => SkTyEmpty
+  | TySum A B => SkTySum (skeletize_vtype A) (skeletize_vtype B)
+  | TyProd A B => SkTyProd (skeletize_vtype A) (skeletize_vtype B)
   | TyList A => SkTyList (skeletize_vtype A)
   | TyFun A C => SkTyFun (skeletize_vtype A) (skeletize_ctype C)
   | TyHandler C D => SkTyHandler (skeletize_ctype C) (skeletize_ctype D)
@@ -187,25 +187,25 @@ Inductive v_ann : forall Γ v A, has_vtype Γ v A -> sk_val -> Prop :=
     v_ann Γ (Int n) TyInt p (SkInt n)
 | AnnPair Γ v1 v2 A B v1' v2' p1 p2 p:
     v_ann Γ v1 A p1 v1' -> v_ann Γ v2 B p2 v2' ->
-    v_ann Γ (Pair v1 v2) (TyΠ A B) p (SkPair v1' v2')
-| AnnInl Γ v A B v' pl p:
+    v_ann Γ (Pair v1 v2) (TyProd A B) p (SkPair v1' v2')
+| AnnLeft Γ v A B v' pl p:
     v_ann Γ v A pl v' ->
-    v_ann Γ (Inl v) (TyΣ A B) p (SkInl v')
-| AnnInr Γ v A B v' pr p:
+    v_ann Γ (Left v) (TySum A B) p (SkLeft v')
+| AnnRight Γ v A B v' pr p:
     v_ann Γ v B pr v' ->
-    v_ann Γ (Inr v) (TyΣ A B) p (SkInr v')
-| AnnListNil Γ A p:
-    v_ann Γ ListNil (TyList A) p (SkListNil)
-| AnnListCons Γ v1 v2 A v1' v2' p1 p2 p:
+    v_ann Γ (Right v) (TySum A B) p (SkRight v')
+| AnnNil Γ A p:
+    v_ann Γ Nil (TyList A) p (SkNil)
+| AnnCons Γ v1 v2 A v1' v2' p1 p2 p:
     v_ann Γ v1 A p1 v1' -> v_ann Γ v2 (TyList A) p2 v2' ->
-    v_ann Γ (ListCons v1 v2) (TyList A) p (SkListCons v1' v2')
+    v_ann Γ (Cons v1 v2) (TyList A) p (SkCons v1' v2')
 | AnnFun Γ c A C c' pc p:
     c_ann (CtxU Γ A) c C pc c' ->
     v_ann Γ (Fun c) (TyFun A C) p (SkFun c')
 | AnnHandler Γ c c' h h' A Σ E D pc ph p:
     c_ann (CtxU Γ A) c D pc c' -> h_ann Γ h Σ D ph h' ->
     v_ann Γ (Handler c h) (TyHandler (CTy A Σ E) D) p (SkHandler c' h')
-| AnnVSubtype Γ v v' A A' p p':
+| AnnVSTy Γ v v' A A' p p':
     v_ann Γ v A p' v' ->
     vsubtype A A' ->
     v_ann Γ v A' p v'
@@ -215,22 +215,22 @@ with c_ann : forall Γ c C, has_ctype Γ c C -> sk_comp -> Prop :=
     v_ann Γ v A pv v' ->
     c_ann Γ (Ret v) (CTy A SigØ EqsØ) p (SkRet v')
 | AnnAbsurd Γ v v' C pv p :
-    v_ann Γ v TyØ pv v' ->
+    v_ann Γ v TyEmpty pv v' ->
     c_ann Γ (Absurd v) C p (SkAbsurd v')
-| AnnΠMatch Γ v v' A B c c' C pv pc p:
-    v_ann Γ v (TyΠ A B) pv v' -> c_ann (CtxU (CtxU Γ A) B) c C pc c'->
-    c_ann Γ (ΠMatch v c) C p (SkΠMatch v' c')
-| AnnΣMatch Γ v v' A B c1 c1' c2 c2' C p pv pc1 pc2:
-    v_ann Γ v (TyΣ A B) pv v' ->
+| AnnProdMatch Γ v v' A B c c' C pv pc p:
+    v_ann Γ v (TyProd A B) pv v' -> c_ann (CtxU (CtxU Γ A) B) c C pc c'->
+    c_ann Γ (ProdMatch v c) C p (SkProdMatch v' c')
+| AnnSumMatch Γ v v' A B c1 c1' c2 c2' C p pv pc1 pc2:
+    v_ann Γ v (TySum A B) pv v' ->
     c_ann (CtxU Γ A) c1 C pc1 c1' -> c_ann (CtxU Γ B) c2 C pc2 c2' ->
-    c_ann Γ (ΣMatch v c1 c2) C p (SkΣMatch v' c1' c2')
+    c_ann Γ (SumMatch v c1 c2) C p (SkSumMatch v' c1' c2')
 | AnnListMatch Γ v v' A c1 c1' c2 c2' C p pv pc1 pc2:
     v_ann Γ v (TyList A) pv v' ->
     c_ann Γ c1 C pc1 c1' -> c_ann (CtxU (CtxU Γ A) (TyList A)) c2 C pc2 c2' ->
     c_ann Γ (ListMatch v c1 c2) C p (SkListMatch v' c1' c2')
-| AnnDoBind Γ c1 c1' c2 c2' A B Σ E p pc1 pc2:
+| AnnDo Γ c1 c1' c2 c2' A B Σ E p pc1 pc2:
     c_ann Γ c1 (CTy A Σ E) pc1 c1' -> c_ann (CtxU Γ A) c2 (CTy B Σ E) pc2 c2' ->
-    c_ann Γ (DoBind c1 c2) (CTy B Σ E) p (SkDoBind c1' c2')
+    c_ann Γ (Do c1 c2) (CTy B Σ E) p (SkDo c1' c2')
 | AnnApp Γ v1 v1' v2 v2' A C pv1 pv2 p:
     v_ann Γ v1 (TyFun A C) pv1 v1' -> v_ann Γ v2 A pv2 v2' ->
     c_ann Γ (App v1 v2) C p (SkApp v1' v2')
@@ -246,7 +246,7 @@ with c_ann : forall Γ c C, has_ctype Γ c C -> sk_comp -> Prop :=
     v_ann Γ v Aop pv v' -> c_ann (CtxU Γ Bop) c (CTy A Σ E) pc c' ->
     c_ann Γ (Op op v c) (CTy A Σ E) p 
       (SkOp op (skeletize_vtype Aop) (skeletize_vtype Bop) v' c')
-| AnnCSubtype Γ c c' C C' p p':
+| AnnCSTy Γ c c' C C' p p':
     c_ann Γ c C p' c' ->
     csubtype C C' ->
     c_ann Γ c C' p c'
